src/Specific/IntegrationTestDisplayCommon.v
@@ -21,9 +21,15 @@ Ltac display_helper f :=
     => let x := fresh "x" in
        lazymatch (eval hnf in A) with
        | @sig ?A ?P
-         => refine (fun x : A => _);
-            let f' := open_constr:(f (exist P x _)) in
-            display_helper f'
+         => lazymatch (eval hnf in A) with
+            | sig _
+              => let f' := open_constr:(fun x : A => f (exist P x _)) in
+                 display_helper f'
+            | _
+              => refine (fun x : A => _);
+                 let f' := open_constr:(f (exist P x _)) in
+                 display_helper f'
+            end
        | _
          => lazymatch A with
             | prod ?A ?B
@@ -35,7 +41,11 @@ Ltac display_helper f :=
                  display_helper f'
             end
        end
-  | sig _ => refine (proj1_sig f)
+  | @sig ?A _
+    => lazymatch (eval hnf in A) with
+       | sig _ => display_helper (proj1_sig f)
+       | _ => refine (proj1_sig f)
+       end
   | _
     => lazymatch t with
        | prod _ _
@@ -53,6 +63,7 @@ Tactic Notation "display" open_constr(f) :=
                                Tuple.map Tuple.map'
                                Lift.lift1_sig Lift.lift2_sig Lift.lift3_sig Lift.lift4_sig Lift.lift4_sig_sig
                                MapProjections.proj2_sig_map Associativity.sig_sig_assoc
+                               sig_conj_by_impl2
                                sig_eq_trans_exist1 sig_R_trans_exist1 sig_eq_trans_rewrite_fun_exist1
                                sig_R_trans_rewrite_fun_exist1
                                adjust_tuple2_tuple2_sig
